ecoop17/dot_storeless_wfrel.v
@@ -26,17 +26,14 @@ Lemma R_env_mon: forall G env m n,
     R_env n env G ->
     m <= n ->
     R_env m env G.
-Proof.
-  intros * Henv; induction Henv; eauto.
-Qed.
+Proof. intros * Henv; induction Henv; eauto. Qed.
 Hint Resolve R_env_mon.
 
 Lemma wf_length : forall k vs ts,
                     R_env k vs ts ->
                     (length vs = length ts).
-Proof.
-  intros * H; induction H; simpl; congruence.
-Qed.
+Proof. intros * H; induction H; simpl; congruence. Qed.
+Hint Resolve wf_length.
 
 Hint Constructors Forall.
 
@@ -45,52 +42,10 @@ Program Definition etp T k e :=
 
 Lemma etp_closed: forall T k v,
     etp T k v -> @wf ty [] T.
-Proof.
-  unfold etp; intros; simp expr_sem in *; tauto.
-Qed.
+Proof. unfold etp; intros; simp expr_sem in *; tauto. Qed.
 Hint Resolve etp_closed.
 
 Hint Rewrite map_length.
-
-Program Definition evalTo env e v k j (HwfE : tm_closed 0 (length env) e) :=
-  steps (tm_subst_all_tot 0 (map VObj env) e _) v j /\ irred v /\ j <= k.
-Solve Obligations with program_simpl; rewrite map_length; auto.
-
-Program Definition vtpEnvCore T k v env (HwfT : wf env T) :=
-  vtp (subst_all_tot 0 (map VObj env) T _) k v.
-Solve Obligations with program_simpl; rewrite map_length; auto.
-
-Program Definition vtpEnv T k v env :=
-  tm_closed 0 0 v /\
-  { HwfT : wf env T | vtpEnvCore T k v env _ }.
-
-Lemma vtpEnv_closed:
-  forall T k v env, vtpEnv T k v env -> wf env T.
-Proof. unfold vtpEnv; program_simpl. Qed.
-Hint Resolve vtpEnv_closed.
-
-Program Definition etpEnvCore T k e env
-        (HwfE : tm_closed 0 (length env) e)
-        (HwfT : wf env T): Prop :=
-  forall v j,
-    evalTo env e v k j _ ->
-    vtpEnvCore T (k - j) v env _.
-Hint Transparent wf.
-
-Program Definition etpEnv T k e env :=
-  { HwfT : wf env T |
-    { HwfE : tm_closed 0 (length env) e | etpEnvCore T k e env _ _ }}.
-Hint Unfold etpEnv.
-Hint Transparent etpEnv.
-Hint Transparent wf.
-
-Lemma etpEnv_closed: forall T k v env,
-    etpEnv T k v env -> wf env T.
-Proof. unfold etpEnv; program_simpl. Qed.
-Hint Resolve etpEnv_closed.
-
-Definition evalToSome env e v k j :=
-  (exists t', tm_subst_all (map VObj env) e = Some t' /\ steps t' v j) /\ irred v /\ j <= k.
 
 Definition vtpEnvSomeCore T k v env :=
   exists T', subst_all (map VObj env) T = Some T' /\
@@ -116,55 +71,6 @@ Lemma etpEnvSome_closed: forall T k v env,
     etpEnvSome T k v env -> wf env T.
 Proof. unfold etpEnvSome; program_simpl. Qed.
 Hint Resolve etpEnvSome_closed.
-
-(* Semantic typing *)
-Program Definition sem_type (G : tenv) (T : ty) (e: tm) :=
-  { HwfT : wf G T | { HwfE : tm_closed 0 (length G) e |
-      forall k env (Henv: R_env k env G), etpEnvCore T k e env _ _ }}.
-Solve Obligations with program_simpl; unfold wf in *; erewrite wf_length in *; eauto.
-
-Program Definition sem_subtype (G : tenv) (T1 T2: ty) :=
-  { HwfT1 : wf G T1 |
-    { HwfT2 : wf G T2 |
-      forall e (HwfE : tm_closed 0 (length G) e),
-      forall k env (Henv : R_env k env G),
-        etpEnvCore T1 k e env _ _ -> etpEnvCore T2 k e env _ _ }}.
-Solve Obligations with program_simpl; unfold wf in *; erewrite wf_length in *; eauto.
-
-Program Definition sem_vl_subtype (G : tenv) (T1 T2: ty) :=
-  { HwfT1 : wf G T1 |
-    { HwfT2 : wf G T2 |
-      forall e (HwfE : tm_closed 0 (length G) e),
-      forall k env (Henv : R_env k env G),
-        vtpEnvCore T1 k e env _ -> vtpEnvCore T2 k e env _ }}.
-Solve Obligations with program_simpl; unfold wf in *; erewrite wf_length in *; eauto.
-
-Lemma sem_type_closed : forall G T e,
-    sem_type G T e -> wf G T.
-Proof. unfold sem_type; program_simpl. Qed.
-
-Lemma sem_subtype_closed1 : forall G T1 T2,
-    sem_subtype G T1 T2 -> wf G T1.
-Proof. unfold sem_subtype; program_simpl. Qed.
-
-Lemma sem_subtype_closed2 : forall G T1 T2,
-    sem_subtype G T1 T2 -> wf G T2.
-Proof. unfold sem_subtype; program_simpl. Qed.
-
-Lemma sem_vl_subtype_closed1 : forall G T1 T2,
-    sem_vl_subtype G T1 T2 -> wf G T1.
-Proof. unfold sem_vl_subtype; program_simpl. Qed.
-
-Lemma sem_vl_subtype_closed2 : forall G T1 T2,
-    sem_vl_subtype G T1 T2 -> wf G T2.
-Proof. unfold sem_vl_subtype; program_simpl. Qed.
-
-Hint Resolve sem_type_closed
-     sem_subtype_closed1
-     sem_subtype_closed2
-     sem_vl_subtype_closed1
-     sem_vl_subtype_closed2.
-Hint Resolve wf_length.
 
 Definition sem_type_some (G : tenv) (T : ty) (e: tm) :=
   wf G T /\ tm_closed 0 (length G) e /\
@@ -208,73 +114,11 @@ Hint Resolve sem_type_some_closed
      sem_vl_subtype_some_closed1
      sem_vl_subtype_some_closed2.
 
-(* Deal with irrelevance of local closure proofs.
-Credits to @Cypi on IRC, see gen_safe_proof and unify_lt_proofs
-https://github.com/cmangin/template-coq/blob/8b3e6ecec085bab8ebe087af07c3db8e56e8aac2/template-coq/theories/Rtree.v#L108-L118
-https://github.com/cmangin/template-coq/blob/8b3e6ecec085bab8ebe087af07c3db8e56e8aac2/template-coq/theories/Rtree.v#L161-L167
- *)
-
-Ltac aux_gen_irr_proof P :=
-  tryif is_var P then fail else
-    let HPs := fresh "Hs" in
-    generalize P as HPs; intro.
-Ltac aux_rem_irr_proof H P :=
-  tryif is_var P then fail else
-    let HPs := fresh "HPs" in
-    let Heqs := fresh "Heqs" in
-    remember P as HPs eqn:Heqs; clear Heqs.
-Ltac prove_closed_irrelevance := eauto using closed_irrelevance, tm_closed_irrelevance, vr_closed_irrelevance, dm_closed_irrelevance, dms_closed_irrelevance.
-Ltac prove_tm_closed_irrelevance := apply tm_closed_irrelevance.
-Ltac unify_tm_closed_proofs :=
-  repeat match goal with
-         | H1 : tm_closed ?i ?k ?T, H2 : tm_closed ?i ?k ?T |- _ =>
-           assert (H1 = H2) as -> by prove_tm_closed_irrelevance
-         end.
-Ltac unify_closed_proofs :=
-  repeat match goal with
-         | H1 : closed ?i ?k ?T, H2 : closed ?i ?k ?T |- _ =>
-           assert (H1 = H2) as -> by prove_closed_irrelevance
-         end.
-
-Ltac gen_irr_proofs :=
-  repeat (reduce_indexTot; match goal with
-         | |- context [ vtpEnvCore _ _ _ _ ?H] => aux_gen_irr_proof H; unfold wf in *
-         | H : context [ vtpEnvCore _ _ _ _ ?P ] |- _ => aux_rem_irr_proof H P; unfold wf in *
-         | H : context [ evalTo _ _ _ _ _ ?P ] |- _ => aux_rem_irr_proof H P
-         end).
-
 Ltac lenG_to_lenEnv :=
   try match goal with
   | H: R_env _ ?env ?G |- _ =>
     replace (length G) with (length env) in * by (eauto using wf_length)
   end.
-
-Ltac remove_irrelevant_localClosure_mismatches :=
-  gen_irr_proofs; lenG_to_lenEnv; unify_tm_closed_proofs; unify_closed_proofs.
-
-Ltac evp := repeat match goal with
-                    | H: exists _, _ |- _ => destruct H
-                    | H: {_ : _ | _} |- _ =>
-                      let x := fresh "x" in
-                      let H' := fresh "H" in
-                      destruct H as [x H']
-                    | H: {_ : _ & _} |- _ => destruct H
-                    | H: _ /\  _ |- _ => destruct H
-                   end.
-
-Lemma evalToRes_closed: forall env e v n k j H,
-    evalTo env e v n j H ->
-    Forall (dms_closed 0 (S k)) env ->
-    tm_closed 0 k v.
-Proof.
-  intros; destruct subst_all_res_closed_rec; ev.
-  unfold evalTo in *; ev.
-  repeat (match goal with
-         | H : context [ tm_subst_all_tot _ _ _ ?P ] |- _ => aux_rem_irr_proof H P; unfold wf in *
-         end).
-  eauto using steps_closed, dms_to_env_closed.
-Qed.
-Hint Resolve evalToRes_closed.
 
 Lemma env_dms_closed: forall k env G l, R_env k env G -> length env = l -> Forall (dms_closed 0 (S l)) env.
 Proof.
@@ -282,47 +126,6 @@ Proof.
   assert (tm_closed 0 0 (tvar (VObj a))) by (eauto using vtp_v_closed); repeat inverts_closed; eauto.
 Qed.
 Hint Resolve env_dms_closed.
-
-Lemma evalToSomeRes_closed: forall env e v n k j l,
-    evalToSome env e v n j ->
-    tm_closed 0 l e ->
-    length env = l ->
-    Forall (dms_closed 0 (S k)) env ->
-    tm_closed 0 k v.
-Proof.
-  unfold evalToSome; intros; subst;
-    assert (exists t', tm_subst_all (map VObj env) e = Some t' /\ tm_closed 0 k t')
-    by (eapply tm_subst_all_nonTot_res_closed; try rewrite map_length; eauto); ev;
-      match goal with
-      | H1 : ?t = Some ?x1, H2 : ?t = Some ?x2 |- _ =>
-        assert (x1 = x2) as -> by congruence
-      end;
-      eauto using steps_closed.
-Qed.
-Hint Resolve evalToSomeRes_closed.
-
-(* Write lemmas to get rid of all the extra side conditions and get to the meat. *)
-Program Lemma vl_subtype_to_subtype : forall G T1 T2,
-    sem_vl_subtype G T1 T2 -> sem_subtype G T1 T2.
-Proof.
-  unfold sem_subtype, sem_vl_subtype, wf.
-  (* intros; evp. *)
-  intros * (? & ? & Hvl).
-  repeat match goal with
-         | H: ?P |- { H : ?P | ?Q } => exists H
-         end.
-  intros * HeVtpT1; unfold etpEnvCore in *.
-  ev; split_conj; intros.
-
-  assert (Forall (dms_closed 0 (S (length env))) env) by eauto using env_dms_closed.
-  assert (HwfV: tm_closed 0 (length env) v) by eauto.
-  assert (HwfV2: tm_closed 0 (length G) v) by (erewrite <- wf_length; eauto).
-  assert (Henvkj: R_env (k - j) env G) by eauto.
-  specialize (Hvl _ HwfV2 (k - j) env Henvkj).
-  specialize (HeVtpT1 v j).
-  remove_irrelevant_localClosure_mismatches; eauto.
-Qed.
-Hint Resolve vl_subtype_to_subtype.
 
 Lemma vl_subtype_some_to_subtype_some : forall G T1 T2
     (Hsub: sem_vl_subtype_some G T1 T2), sem_subtype_some G T1 T2.
