ecoop17/dot_storeless_wfrel_sigma.v
@@ -1,0 +1,179 @@
+Require Import Omega.
+Require Import Equations.Equations.
+Require Import tactics.
+
+Require Import dot_storeless_tidy.
+Require Import dot_storeless_subst_aux.
+Require Import dot_storeless_wfrel_aux.
+Require Import tactics.
+
+Require Import dot_storeless_wfrel.
+
+Program Definition evalTo env e v k j (HwfE : tm_closed 0 (length env) e) :=
+  steps (tm_subst_all_tot 0 (map VObj env) e _) v j /\ irred v /\ j <= k.
+Solve Obligations with program_simpl; rewrite map_length; auto.
+
+Program Definition vtpEnvCore T k v env (HwfT : wf env T) :=
+  vtp (subst_all_tot 0 (map VObj env) T _) k v.
+Solve Obligations with program_simpl; rewrite map_length; auto.
+
+Program Definition vtpEnv T k v env :=
+  tm_closed 0 0 v /\
+  { HwfT : wf env T | vtpEnvCore T k v env _ }.
+
+Lemma vtpEnv_closed:
+  forall T k v env, vtpEnv T k v env -> wf env T.
+Proof. unfold vtpEnv; program_simpl. Qed.
+Hint Resolve vtpEnv_closed.
+
+Program Definition etpEnvCore T k e env
+        (HwfE : tm_closed 0 (length env) e)
+        (HwfT : wf env T): Prop :=
+  forall v j,
+    evalTo env e v k j _ ->
+    vtpEnvCore T (k - j) v env _.
+Hint Transparent wf.
+
+Program Definition etpEnv T k e env :=
+  { HwfT : wf env T |
+    { HwfE : tm_closed 0 (length env) e | etpEnvCore T k e env _ _ }}.
+Hint Unfold etpEnv.
+Hint Transparent etpEnv.
+Hint Transparent wf.
+
+Lemma etpEnv_closed: forall T k v env,
+    etpEnv T k v env -> wf env T.
+Proof. unfold etpEnv; program_simpl. Qed.
+Hint Resolve etpEnv_closed.
+
+(* Semantic typing *)
+Program Definition sem_type (G : tenv) (T : ty) (e: tm) :=
+  { HwfT : wf G T | { HwfE : tm_closed 0 (length G) e |
+      forall k env (Henv: R_env k env G), etpEnvCore T k e env _ _ }}.
+Solve Obligations with program_simpl; unfold wf in *; erewrite wf_length in *; eauto.
+
+Program Definition sem_subtype (G : tenv) (T1 T2: ty) :=
+  { HwfT1 : wf G T1 |
+    { HwfT2 : wf G T2 |
+      forall e (HwfE : tm_closed 0 (length G) e),
+      forall k env (Henv : R_env k env G),
+        etpEnvCore T1 k e env _ _ -> etpEnvCore T2 k e env _ _ }}.
+Solve Obligations with program_simpl; unfold wf in *; erewrite wf_length in *; eauto.
+
+Program Definition sem_vl_subtype (G : tenv) (T1 T2: ty) :=
+  { HwfT1 : wf G T1 |
+    { HwfT2 : wf G T2 |
+      forall e (HwfE : tm_closed 0 (length G) e),
+      forall k env (Henv : R_env k env G),
+        vtpEnvCore T1 k e env _ -> vtpEnvCore T2 k e env _ }}.
+Solve Obligations with program_simpl; unfold wf in *; erewrite wf_length in *; eauto.
+
+Lemma sem_type_closed : forall G T e,
+    sem_type G T e -> wf G T.
+Proof. unfold sem_type; program_simpl. Qed.
+
+Lemma sem_subtype_closed1 : forall G T1 T2,
+    sem_subtype G T1 T2 -> wf G T1.
+Proof. unfold sem_subtype; program_simpl. Qed.
+
+Lemma sem_subtype_closed2 : forall G T1 T2,
+    sem_subtype G T1 T2 -> wf G T2.
+Proof. unfold sem_subtype; program_simpl. Qed.
+
+Lemma sem_vl_subtype_closed1 : forall G T1 T2,
+    sem_vl_subtype G T1 T2 -> wf G T1.
+Proof. unfold sem_vl_subtype; program_simpl. Qed.
+
+Lemma sem_vl_subtype_closed2 : forall G T1 T2,
+    sem_vl_subtype G T1 T2 -> wf G T2.
+Proof. unfold sem_vl_subtype; program_simpl. Qed.
+
+Hint Resolve sem_type_closed
+     sem_subtype_closed1
+     sem_subtype_closed2
+     sem_vl_subtype_closed1
+     sem_vl_subtype_closed2.
+
+(* Deal with irrelevance of local closure proofs.
+Credits to @Cypi on IRC, see gen_safe_proof and unify_lt_proofs
+https://github.com/cmangin/template-coq/blob/8b3e6ecec085bab8ebe087af07c3db8e56e8aac2/template-coq/theories/Rtree.v#L108-L118
+https://github.com/cmangin/template-coq/blob/8b3e6ecec085bab8ebe087af07c3db8e56e8aac2/template-coq/theories/Rtree.v#L161-L167
+ *)
+
+Ltac aux_gen_irr_proof P :=
+  tryif is_var P then fail else
+    let HPs := fresh "Hs" in
+    generalize P as HPs; intro.
+Ltac aux_rem_irr_proof H P :=
+  tryif is_var P then fail else
+    let HPs := fresh "HPs" in
+    let Heqs := fresh "Heqs" in
+    remember P as HPs eqn:Heqs; clear Heqs.
+Ltac prove_closed_irrelevance := eauto using closed_irrelevance, tm_closed_irrelevance, vr_closed_irrelevance, dm_closed_irrelevance, dms_closed_irrelevance.
+Ltac prove_tm_closed_irrelevance := apply tm_closed_irrelevance.
+Ltac unify_tm_closed_proofs :=
+  repeat match goal with
+         | H1 : tm_closed ?i ?k ?T, H2 : tm_closed ?i ?k ?T |- _ =>
+           assert (H1 = H2) as -> by prove_tm_closed_irrelevance
+         end.
+Ltac unify_closed_proofs :=
+  repeat match goal with
+         | H1 : closed ?i ?k ?T, H2 : closed ?i ?k ?T |- _ =>
+           assert (H1 = H2) as -> by prove_closed_irrelevance
+         end.
+
+Ltac gen_irr_proofs :=
+  repeat (reduce_indexTot; match goal with
+         | |- context [ vtpEnvCore _ _ _ _ ?H] => aux_gen_irr_proof H; unfold wf in *
+         | H : context [ vtpEnvCore _ _ _ _ ?P ] |- _ => aux_rem_irr_proof H P; unfold wf in *
+         | H : context [ evalTo _ _ _ _ _ ?P ] |- _ => aux_rem_irr_proof H P
+         end).
+
+Ltac remove_irrelevant_localClosure_mismatches :=
+  gen_irr_proofs; lenG_to_lenEnv; unify_tm_closed_proofs; unify_closed_proofs.
+
+Ltac evp := repeat match goal with
+                    | H: exists _, _ |- _ => destruct H
+                    | H: {_ : _ | _} |- _ =>
+                      let x := fresh "x" in
+                      let H' := fresh "H" in
+                      destruct H as [x H']
+                    | H: {_ : _ & _} |- _ => destruct H
+                    | H: _ /\  _ |- _ => destruct H
+                   end.
+
+Lemma evalToRes_closed: forall env e v n k j H,
+    evalTo env e v n j H ->
+    Forall (dms_closed 0 (S k)) env ->
+    tm_closed 0 k v.
+Proof.
+  intros; destruct subst_all_res_closed_rec; ev.
+  unfold evalTo in *; ev.
+  repeat (match goal with
+         | H : context [ tm_subst_all_tot _ _ _ ?P ] |- _ => aux_rem_irr_proof H P; unfold wf in *
+         end).
+  eauto using steps_closed, dms_to_env_closed.
+Qed.
+Hint Resolve evalToRes_closed.
+
+Program Lemma vl_subtype_to_subtype : forall G T1 T2,
+    sem_vl_subtype G T1 T2 -> sem_subtype G T1 T2.
+Proof.
+  unfold sem_subtype, sem_vl_subtype, wf.
+  (* intros; evp. *)
+  intros * (? & ? & Hvl).
+  repeat match goal with
+         | H: ?P |- { H : ?P | ?Q } => exists H
+         end.
+  intros * HeVtpT1; unfold etpEnvCore in *.
+  ev; split_conj; intros.
+
+  assert (Forall (dms_closed 0 (S (length env))) env) by eauto using env_dms_closed.
+  assert (HwfV: tm_closed 0 (length env) v) by eauto.
+  assert (HwfV2: tm_closed 0 (length G) v) by (erewrite <- wf_length; eauto).
+  assert (Henvkj: R_env (k - j) env G) by eauto.
+  specialize (Hvl _ HwfV2 (k - j) env Henvkj).
+  specialize (HeVtpT1 v j).
+  remove_irrelevant_localClosure_mismatches; eauto.
+Qed.
+Hint Resolve vl_subtype_to_subtype.
